Translation.v
@@ -1,12 +1,16 @@
 Add LoadPath "vst".
 Require Import CpdtTactics.
 Require Import Types.
+Import HE.
 Require Import Language.
 Require Export ProgramLogic.
 Require Import Subst.
 Require Import List.
 Import ListNotations.
 Require Import Coq.Unicode.Utf8.
+Require Import msl.eq_dec.
+
+Instance EQ_EQUIVALENCE : Equivalence (@eq assert) := _.
 
 Set Implicit Arguments.
 
@@ -40,17 +44,25 @@ Fixpoint sep_env (Γ : type_env) : assert :=
     | (x,t) :: Γ' => sep_ty (var_e x) t && sep_env Γ'
   end && emp.
 
-Definition sep_heap_bind l x t :=
-  !!(runloc l = null) 
-    || (emapsto (addr_v (runloc l)) (var_e x)
-        * sep_ty (var_e x) t).
+Definition sep_heap_bind l (xt : type_binding) :=
+  let (x, t) := xt in
+      !!(runloc l = null) 
+        || (emapsto (addr_v (runloc l)) (var_e x)
+            * sep_ty (var_e x) t).
 
-Fixpoint sep_heap (Σ : heap_env) : assert :=
-  match Σ with
+Fixpoint sep_heap' es :=
+  match es with
     | nil => emp
-    | (l, (x, t))::Σ' =>
-      sep_heap_bind l x t * sep_heap Σ'
+    | (l, xt) :: es' => sep_heap_bind l xt * sep_heap' es'
   end.
+
+Definition sep_heap (Σ : heap_env)  : assert :=
+  fold (fun l xt a =>
+          sep_heap_bind l xt * a) Σ emp.
+  (* sep_heap' (elements Σ). *)
+  (* fold (fun _ xt a => xt * a) *)
+  (*   (mapi (fun l xt => sep_heap_bind l xt) Σ) *)
+  (*   emp. *)
 
 Fixpoint sep_guards (Δ : guards) : assert :=
   match Δ with
@@ -102,7 +114,7 @@ Lemma sep_ty_pure :
 Proof.
   intros.
   unfold pure, sep_ty.
-  destruct t.
+  destruct t0.
   do 2 apply andp_left1.
   apply sep_base_pure.
 Qed.
@@ -148,130 +160,168 @@ Ltac purity :=
       (apply andp_left1; purity || apply andp_left2; purity)
   end.
 
-Lemma sep_heap_app :
-  forall H1 H2,
-    sep_heap (H1 ++ H2) = sep_heap H1 * sep_heap H2.
-Proof.
-  induction H1 as [| (l, (x,t))].
-  + intros. 
-    simpl.
-    extensionality.
-    rewrite sepcon_comm.
-    rewrite sepcon_emp.
-    reflexivity.
-  + intros. 
-    rewrite <- app_comm_cons.
-    unfold sep_heap. fold sep_heap.
-    rewrite IHlist.
-    rewrite sepcon_assoc.
-    reflexivity.
-Qed.
-
-Lemma sep_heap_decompose' :
-  forall H l x t, 
-    In (l, (x, t)) H -> 
-    exists H', (sep_heap H = sep_heap_bind l x t * sep_heap H'
-                /\ (forall l', l <> l' -> (loc_in l' H <-> loc_in l' H'))).
-Proof.
-  induction H as [ | [l' [x' t']]].
-  + intros. contradiction H. 
-  + intros. destruct H0. 
-    * inv H0.
-      unfold sep_heap at 1; fold sep_heap.
-      exists H. repeat split. 
-      intro.
-      unfold loc_in in *.
-      destruct H1. destruct H1. inv H1. congruence.
-      exists x0. assumption.
-      unfold loc_in.
-      intros [xt]. intro.
-      exists xt. eauto with datatypes.
-    * specialize (IHlist l x t H0). 
-      destruct IHlist as [ H'' ].
-      destruct H1 as [A B].
-      unfold sep_heap; fold sep_heap.
-      rewrite A.
-      rewrite <- sepcon_assoc.
-      exists ((l',(x',t'))::H'').
-      unfold sep_heap; fold sep_heap.
-      rewrite <- sepcon_assoc.
-      split.
-        { f_equal.
-          rewrite sepcon_comm.
-          reflexivity. }
-        { repeat split. 
-          intros.
-          unfold loc_in in *.
-          destruct H2. destruct H2. inv H2. exists (x', t'). left. reflexivity.
-          specialize (B l'0 H1). destruct B. 
-          destruct H3. exists x0. assumption.
-          exists x1. right. assumption.
+(* Lemma sep_heap_decompose' : *)
+(*   forall H l x t,  *)
+(*     in (l, (x, t)) H ->  *)
+(*     exists H', (sep_heap H = sep_heap_bind l x t * sep_heap H' *)
+(*                 /\ (forall l', l <> l' -> (loc_in l' H <-> loc_in l' H'))). *)
+(* Proof. *)
+(*   induction H as [ | [l' [x' t']]]. *)
+(*   + intros. contradiction H.  *)
+(*   + intros. destruct H0.  *)
+(*     * inv H0. *)
+(*       unfold sep_heap at 1; fold sep_heap. *)
+(*       exists H. repeat split.  *)
+(*       intro. *)
+(*       unfold loc_in in *. *)
+(*       destruct H1. destruct H1. inv H1. congruence. *)
+(*       exists x0. assumption. *)
+(*       unfold loc_in. *)
+(*       intros [xt]. intro. *)
+(*       exists xt. eauto with datatypes. *)
+(*     * specialize (IHlist l x t H0).  *)
+(*       destruct IHlist as [ H'' ]. *)
+(*       destruct H1 as [A B]. *)
+(*       unfold sep_heap; fold sep_heap. *)
+(*       rewrite A. *)
+(*       rewrite <- sepcon_assoc. *)
+(*       exists ((l',(x',t'))::H''). *)
+(*       unfold sep_heap; fold sep_heap. *)
+(*       rewrite <- sepcon_assoc. *)
+(*       split. *)
+(*         { f_equal. *)
+(*           rewrite sepcon_comm. *)
+(*           reflexivity. } *)
+(*         { repeat split.  *)
+(*           intros. *)
+(*           unfold loc_in in *. *)
+(*           destruct H2. destruct H2. inv H2. exists (x', t'). left. reflexivity. *)
+(*           specialize (B l'0 H1). destruct B.  *)
+(*           destruct H3. exists x0. assumption. *)
+(*           exists x1. right. assumption. *)
           
-          intro.
-          unfold loc_in in *.
-          destruct H2. destruct H2. inv H2. exists (x', t'). left. reflexivity.
-          specialize (B l'0 H1). destruct B.
-          destruct H4. exists x0. assumption.
-          exists x1. right. assumption. }
+(*           intro. *)
+(*           unfold loc_in in *. *)
+(*           destruct H2. destruct H2. inv H2. exists (x', t'). left. reflexivity. *)
+(*           specialize (B l'0 H1). destruct B. *)
+(*           destruct H4. exists x0. assumption. *)
+(*           exists x1. right. assumption. } *)
+(* Qed. *)
+
+(* Lemma sep_heap_split : *)
+(*   forall H H1 H2, *)
+(*     heap_split H1 H2 H -> *)
+(*     sep_heap H = sep_heap H1 * sep_heap H2. *)
+(* Proof. *)
+(*   intros H. *)
+(*   induction H as [ | (l,xt)]; intros. *)
+(*   + assert (H1 = []) by (eapply heap_split_emp1; eauto). *)
+(*     assert (H2 = []) by (eapply heap_split_emp2; eauto). *)
+(*     subst H1. subst H2. *)
+(*     simpl. rewrite sepcon_emp. reflexivity. *)
+(*   + assert ((l, xt) :: H = [(l, xt)] ++ H) by reflexivity. *)
+(*     rewrite H3. *)
+(*     rewrite sep_heap_app. *)
+(*     destruct xt as [x t]. *)
+(*     unfold sep_heap at 1. *)
+(*     rewrite sepcon_emp. *)
+
+(*     unfold heap_split in H0; decompose [and] H0. *)
+(*     destruct (H9 l (x,t)). left. reflexivity. { *)
+(*       destruct (sep_heap_decompose' H1 l x t) as [H1']. *)
+(*       apply H8. *)
+(*       specialize (IHlist H1' H2). *)
+(*       rewrite IHlist. *)
+(*       destruct H10. *)
+(*       rewrite H10. *)
+(*       rewrite sepcon_assoc. *)
+(*       reflexivity. *)
+
+(*       unfold heap_split. *)
+(*       repeat split. *)
+(*       inv H4. assumption. *)
+
+(*     unfold heap_split in H0. *)
+(*     destruct H0. *)
+(*     specialize (H4 l xt). *)
+(*     destruct H4. left. reflexivity. *)
+(*     pose (sep_heap_decompose' H1 l x t) as H1_decomp. *)
+(*     destruct H1_decomp as [H1']. apply H4.  *)
+(*     specialize (IHlist H1' H2). *)
+(*     destruct H5. *)
+(*     rewrite IHlist. *)
+(*     rewrite H5. *)
+(*     unfold sep_heap; fold sep_heap. *)
+(*     rewrite sepcon_emp. rewrite sepcon_assoc. reflexivity. *)
+    
+(*     unfold heap_split. split. { *)
+(*       intros l0. *)
+(*       repeat rewrite <- loc_in_not_in in *. *)
+(*       intro l0_not_in. *)
+(*       split. intro. *)
+(*       specialize (H6 l0). *)
+(*       specialize (H0 l0). *)
+(*       repeat rewrite <- loc_in_not_in in H0. *)
+(*       destruct H0. *)
+(*       intro. *)
+(*       intros l0. unfold loc_not_in in *. intros A. *)
+(*       split. { *)
+
+Import HE_Props.
+Import HE_Props.F.
+Import HE_Facts.
+
+Lemma sep_heap_split' :
+  forall H A,
+    let f := (fun l xt a => sep_heap_bind l xt * a) in
+    sep_heap H * A = fold f H A.
+Proof.
+  intros.
+  unfold sep_heap.
+  repeat rewrite fold_spec_right.
+  
+  induction (rev (elements H)) as [ | [l [x t]]].
+  simpl.
+  rewrite <- sepcon_emp.
+  rewrite sepcon_comm.
+  extensionality.
+  normalize.
+ 
+  unfold fold_right at 2.
+  unfold fold_right at 2 in IHl.
+  rewrite <- IHl.
+  unfold f.
+  unfold uncurry.
+  simpl. extensionality ρ.
+  rewrite sepcon_assoc.
+  reflexivity.
 Qed.
 
+Corollary sep_heap_split'' :
+  forall H1 H2,
+    let f := (fun l xt a => sep_heap_bind l xt * a) in
+    sep_heap H1 * sep_heap H2 = fold f H1 (sep_heap H2).
+Proof.
+  intros.
+  apply sep_heap_split'.
+Qed.
+        
 Lemma sep_heap_split :
   forall H H1 H2,
-    heap_split H1 H2 H ->
+    heap_split H1 H2 H -> 
     sep_heap H = sep_heap H1 * sep_heap H2.
 Proof.
-  intros H.
-  induction H as [ | (l,xt)]; intros.
-  + assert (H1 = []) by (eapply heap_split_emp1; eauto).
-    assert (H2 = []) by (eapply heap_split_emp2; eauto).
-    subst H1. subst H2.
-    simpl. rewrite sepcon_emp. reflexivity.
-  + assert ((l, xt) :: H = [(l, xt)] ++ H) by reflexivity.
-    rewrite H3.
-    rewrite sep_heap_app.
-    destruct xt as [x t].
-    unfold sep_heap at 1.
-    rewrite sepcon_emp.
-
-    unfold heap_split in H0; decompose [and] H0.
-    destruct (H9 l (x,t)). left. reflexivity. {
-      destruct (sep_heap_decompose' H1 l x t) as [H1'].
-      apply H8.
-      specialize (IHlist H1' H2).
-      rewrite IHlist.
-      destruct H10.
-      rewrite H10.
-      rewrite sepcon_assoc.
-      reflexivity.
-
-      unfold heap_split.
-      repeat split.
-      inv H4. assumption.
-
-    unfold heap_split in H0.
-    destruct H0.
-    specialize (H4 l xt).
-    destruct H4. left. reflexivity.
-    pose (sep_heap_decompose' H1 l x t) as H1_decomp.
-    destruct H1_decomp as [H1']. apply H4. 
-    specialize (IHlist H1' H2).
-    destruct H5.
-    rewrite IHlist.
-    rewrite H5.
-    unfold sep_heap; fold sep_heap.
-    rewrite sepcon_emp. rewrite sepcon_assoc. reflexivity.
-    
-    unfold heap_split. split. {
-      intros l0.
-      repeat rewrite <- loc_in_not_in in *.
-      intro l0_not_in.
-      split. intro.
-      specialize (H6 l0).
-      specialize (H0 l0).
-      repeat rewrite <- loc_in_not_in in H0.
-      destruct H0.
-      intro.
-      intros l0. unfold loc_not_in in *. intros A.
-      split. {
-        
-  
+  unfold heap_split in *.
+  intros.
+  set (f := (fun l xt a => sep_heap_bind l xt * a)).
+  assert (sep_heap H1 * sep_heap H2 = fold f H1 (fold f H2 emp)).
+  apply sep_heap_split''.
+  rewrite H3.
+  apply (Partition_fold (eqA := eq)).
+  apply EQ_EQUIVALENCE.
+  solve_proper.
+  hnf. intros. extensionality. 
+  repeat rewrite <- sepcon_assoc. 
+  rewrite sepcon_comm with (P := sep_heap_bind k e). reflexivity.
+  assumption.
+Qed.
